proof/correctness/BitEncoding_hakyber.ec
@@ -1,43 +1,54 @@
-require import AllCore IntDiv Array256 Array128.
-require import List Ring StdOrder Fq.
-require import IntMin.
-require import List_extra Ring_extra RealExp_extra IntDiv_extra.
-require import List_hakyber IntDiv_hakyber For.
-
-import Fq IntOrder.
-
-import Kyber_.
-import ZModField.
-import BitEncoding.BS2Int.
+require import AllCore StdOrder List BitEncoding StdBigop.
+(*---*) import IntOrder BS2Int Bigint.
 
 
-  op bitrev (i k : int) = bs2int (rev (int2bs i k)).
+op bitrev (i k : int) = bs2int (rev (int2bs i k)).
 
-  lemma bitrev_ineq (i k : int) :
-    0 <= i =>
-    0 <= bitrev i k < 2 ^ i.
-  proof.
-    move => le0i; split; [apply bs2int_ge0|move => _]; rewrite /bitrev; move: (size_int2bs i k) => @/max.
-    by case: (0 < i) => [_ {2}<-|lei0]; [|(have <-: (i = 0) by smt()); move => {2}<-]; rewrite -size_rev; apply bs2int_le2Xs.
-  qed.
+lemma bitrev_neg (i k : int) :
+  i <= 0 =>
+  bitrev i k = 0.
+proof. by rewrite /bitrev => lei0; move: (size_int2bs i k); rewrite ler_maxl // size_eq0 => ->; rewrite rev_nil bs2int_nil. qed.
 
-  lemma bitrev_involutive (i k : int) :
-    0 <= i =>
-    k \in range 0 (2 ^ i) =>
-    bitrev i (bitrev i k) = k.
-  proof.
-    move => le0i /mem_range [le0k ltk2powi] @/bitrev.
-    suff {1}->: i = size (rev (int2bs i k)).
-    - by rewrite bs2intK revK int2bsK.
-    by rewrite size_rev size_int2bs ler_maxr.
-  qed.
+lemma bitrev_0 (i : int) :
+  bitrev i 0 = 0.
+proof.
+  case (0 <= i) => [le0i|/ltrNge /ltzW lei0]; last by rewrite bitrev_neg.
+  rewrite /bitrev int2bs0 rev_nseq /bs2int size_nseq maxrC maxrE.
+  rewrite (BIA.eq_big_seq _ (fun n => 0)) ?BIA.sumri_const -?mulr_intr //= le0i //=.
+  by move => x /mem_range [le0x ltxi]; rewrite nth_nseq.
+qed.
 
-  lemma bitrev_injective (i k1 k2 : int) :
-    0 <= i =>
-    k1 \in range 0 (2 ^ i) =>
-    k2 \in range 0 (2 ^ i) =>
-    bitrev i k1 = bitrev i k2 =>
-    k1 = k2.
-  proof.
-    by move => le0i Hk1in Hk2in eq_bitrev; rewrite -(bitrev_involutive i k1) // -(bitrev_involutive i k2) // eq_bitrev.
-  qed.
+lemma bitrev_range (i k : int) :
+  bitrev i k \in range 0 (2 ^ i).
+proof.
+  case (0 <= i) => [le0i|/ltrNge /ltzW lei0]; last by rewrite bitrev_neg // mem_range /= expr_gt0.
+  rewrite mem_range; split; [apply bs2int_ge0|move => _]; rewrite /bitrev; move: (size_int2bs i k) => @/max.
+  by case: (0 < i) => [_ {2}<-|lei0]; [|(have <-: (i = 0) by smt()); move => {2}<-]; rewrite -size_rev; apply bs2int_le2Xs.
+qed.
+
+lemma bitrev_involutive (i k : int) :
+  0 <= i =>
+  k \in range 0 (2 ^ i) =>
+  bitrev i (bitrev i k) = k.
+proof.
+  move => le0i /mem_range [le0k ltk2powi] @/bitrev.
+  suff {1}->: i = size (rev (int2bs i k)).
+  - by rewrite bs2intK revK int2bsK.
+  by rewrite size_rev size_int2bs ler_maxr.
+qed.
+
+lemma bitrev_injective (i k1 k2 : int) :
+  0 <= i =>
+  k1 \in range 0 (2 ^ i) =>
+  k2 \in range 0 (2 ^ i) =>
+  bitrev i k1 = bitrev i k2 =>
+  k1 = k2.
+proof. by move => le0i Hk1in Hk2in eq_bitrev; rewrite -(bitrev_involutive i k1) // -(bitrev_involutive i k2) // eq_bitrev. qed.
+
+lemma bitrev_bijective (i k1 k2 : int) :
+  0 <= i =>
+  k1 \in range 0 (2 ^ i) =>
+  k2 \in range 0 (2 ^ i) =>
+  bitrev i k1 = bitrev i k2 <=>
+  k1 = k2.
+proof. by move => le0i Hk1in Hk2in; split => [|-> //]; apply bitrev_injective. qed.
