proof/correctness/List_hakyber.ec
@@ -84,3 +84,22 @@ lemma all_range_2_eq P Q (min1 max1 min2 max2 : int) :
   all_range_2 P min1 max1 min2 max2 <=>
   all_range_2 Q min1 max1 min2 max2.
 proof. by move => Heq2; apply all_range_eq => y Hy_range /=; apply all_range_eq => x Hx_range /=; apply Heq2. qed.
+
+
+(*-------------------------------------------*)
+
+lemma range_incl (x min1 max1 min2 max2 : int) :
+  min2 <= min1 =>
+  max1 <= max2 =>
+  x \in range min1 max1 =>
+  x \in range min2 max2.
+proof. by rewrite !mem_range => ? ? [? ?]; split;[apply/(lez_trans min1)|move => _; apply/(ltr_le_trans max1)]. qed.
+
+lemma add_range (x y min1 max1 min2 max2 : int) :
+  x \in range min1 max1 =>
+  y \in range min2 max2 =>
+  x + y \in range (min1 + min2) (max1 + max2 - 1).
+proof. by rewrite !mem_range => -[? ?] [? ?]; rewrite ler_add //= ltr_subr_addl addrA ler_lt_add // lez_add1r. qed.
+
+lemma range_mul x m n a : 0 < a => x \in range m n => x * a \in range (m * a) (n * a).
+proof. by rewrite !mem_range => le0a [? ?]; rewrite ler_pmul2r // ltr_pmul2r. qed.
